Buffer example: C code

theories/examples/buffers.v
@@ -5,7 +5,7 @@ From melocoton Require Import named_props.
 From melocoton.interop Require Import basics basics_resources.
 From melocoton.lang_to_mlang Require Import lang weakestpre.
 From melocoton.interop Require Import lang weakestpre update_laws wp_utils wp_ext_call_laws wp_simulation.
-From melocoton.c_interop Require Import rules.
+From melocoton.c_interop Require Import rules notation.
 From melocoton.ml_lang Require Import notation lang_instantiation.
 From melocoton.c_lang Require Import mlang_instantiation lang_instantiation.
 From melocoton.ml_lang Require proofmode.
@@ -13,6 +13,7 @@ From melocoton.c_lang Require notation proofmode.
 From melocoton.mlanguage Require Import progenv.
 From melocoton.mlanguage Require weakestpre.
 From melocoton.linking Require Import lang weakestpre.
+From melocoton.examples Require Import compression.
 
 
 Section C_prog.
@@ -21,59 +22,88 @@ Import melocoton.c_lang.notation melocoton.c_lang.proofmode.
 Context `{SI:indexT}.
 Context `{!heapG_C Σ, !heapG_ML Σ, !invG Σ, !primitive_laws.heapG_ML Σ, !wrapperG Σ}.
 
-Definition CAMLlocal (n:string) (e : expr) : expr :=
-  (let: n := malloc (#1) in
-    (Var n <- (call: &"int2val" with (Val (#0))));;
-    (call: &"registerroot" with (Var n));; e).
+(** our code differs from the original in the paper as follows:
 
-Notation "'CAMLlocal:' x 'in' e2" := (CAMLlocal x%string e2%CE)
-  (at level 200, x at level 1, e2 at level 200,
-   format "'[' 'CAMLlocal:'  x   'in'  '/' e2 ']'") : c_expr_scope.
+The paper has a record
+------------------
+|used_ref|cap|blk|
+------------------
+  ↓
+------
+|used|
+------
+where used_ref is a reference/mutable field
+
+Since we don't have records, only two-value pairs, our value looks as follows (aux_ref is supposed to be another pair)
+------------------
+|used_ref|aux_ref|
+------------------
+  ↓          ↓
+------   ---------
+|used|   |cap|blk|
+------   ---------
+
+Additionally, we do not CAMLparam/CAMLlocal variables that
+* are integers
+* don't have to survive an allocation
+*)
 
 Definition buf_alloc_code (cap : expr) : expr :=
-  CAMLlocal: "bk" in
-  "bk" <- call: &"allocforeign" with ( ) ;;
-  call: &"writeforeign" with ( *"bk", malloc (call: &"val2int" with (cap))) ;;
-  CAMLlocal: "bf" in
-  "bf" <- call: &"alloc" with (Val #2, Val #0) ;;
-  CAMLlocal: "bf2" in
-  "bf2" <- call: &"alloc" with (Val #2, Val #0) ;;
-  CAMLlocal: "bfref" in
-  "bfref" <- call: &"alloc" with (Val #1, Val #0) ;;
-  call: &"modify" with ( *"bf", Val #0, *"bfref") ;;
-  call: &"modify" with ( *"bf", Val #1, *"bf2") ;;
-  call: &"modify" with ( *"bf2", Val #0, cap ) ;;
-  call: &"modify" with ( *"bf2", Val #1, *"bk") ;;
-  call: &"modify" with ( *"bfref", Val #0, call: &"int2val" with (Val #0) ) ;;
-  call: &"unregisterroot" with ( *"bk" ) ;;
-  call: &"unregisterroot" with ( *"bf" ) ;;
-  call: &"unregisterroot" with ( *"bf2" ) ;;
-  call: &"unregisterroot" with ( *"bfref" ) ;;
-  let: "retval" := *"bf" in
-  free ("bk", #1) ;; free ("bf", #1) ;; free ("bf2", #1) ;; free ("bfref", #1) ;;
-  "retval".
+  CAMLlocal: "bk" in 
+  CAMLlocal: "bf" in 
+  CAMLlocal: "bf2" in 
+  let: "bfref" := malloc (#1) in
+  "bk" <- caml_alloc_custom ( ) ;;
+  Custom_contents ( *"bk" ) :=  Val_int (cap) ;;
+  "bf"    <- caml_alloc (#2, #0) ;;
+  "bf2"   <- caml_alloc (#2, #0) ;;
+  "bfref" <- caml_alloc (#1, #0) ;;
+  Store_field ( &Field( *"bfref", #0), Val_int (#0)) ;;
+  Store_field ( &Field( *"bf", #0), *"bfref") ;;
+  Store_field ( &Field( *"bf", #1), *"bf2") ;;
+  Store_field ( &Field( *"bf2", #0), cap) ;;
+  Store_field ( &Field( *"bf2", #1), *"bk") ;;
+  free ("bfref", #1) ;;
+  CAMLreturn: * "bf" unregistering ["bk", "bf", "bf2", "bfref"].
+Definition buf_alloc_fun := Fun [BNamed "cap"] (buf_alloc_code "cap") .
+Definition buf_alloc_name := "buf_alloc".
+
 
 Definition buf_upd_code (iv jv f_arg bf_arg : expr) : expr :=
-  CAMLlocal: "f" in
-  "f" <- f_arg ;;
-  CAMLlocal: "bf" in
-  "bf" <- bf_arg ;;
-  let: "bts" := call: &"readforeign" with (
-      call: &"readfield" with ( call: &"readfield" with ( *"bf", Val #1), Val #1)) in
-  let: "j" := call: &"val2int" with ( jv ) in
+  CAMLlocal: "f" in "f" <- f_arg ;;
+  CAMLlocal: "bf" in "bf" <- bf_arg ;;
+  let: "bts" := Custom_contents(Field(Field("bf", #1), #1)) in
+  let: "j" := Int_val ( jv ) in
   let: "i" := malloc ( #1 ) in
-  "i" <- call: &"val2int" with ( iv ) ;;
+  "i" <- Int_val ( iv ) ;;
   while: * "i" ≤ "j" do
-    ( "bts" +ₗ ( *"i") <- call: &"val2int" with (call: &"callback" with ( *"f", call: &"int2val" with ( *"i"))) ;;
-      if: (call: &"val2int" with (call: &"readfield" with (call: &"readfield" with ( *"bf", Val #0), Val #0)) < *"i" + #1)
-      then (call: &"modify" with (call: &"readfield" with ( *"bf", Val #0), Val #0, call: &"int2val" with ( *"i" + #1)))
+    ( "bts" +ₗ ( *"i") <- Int_val (call: &"callback" with ( *"f", Val_int ( *"i"))) ;;
+      if: Int_val(Field(Field("bf", #0), #0)) < *"i" + #1
+      then Store_field (&Field(Field("bf", #0), #0), Val_int ( *"i" + #1))
       else Skip ;;
       "i" <- *"i" + #1 ) ;;
-  call: &"unregisterroot" with ( *"f" ) ;;
-  call: &"unregisterroot" with ( *"bf" ) ;;
-  free ("f", #1);; free ("bf", #1);; free ("i", #1) ;;
-  call: &"int2val" with (Val #0).
-  
+  free ("i", #1);;
+  CAMLreturn: Int_val (#0) unregistering ["f", "bf"].
+Definition buf_upd_fun := Fun [BNamed "iv"; BNamed "jv"; BNamed "f_arg"; BNamed "bf_arg"]
+                              (buf_upd_code "iv" "jv" "f_arg" "bf_arg").
+Definition buf_upd_name := "buf_upd".
+
+Definition wrap_max_len_code (i : expr) :=
+  (Val_int (call: &buffy_max_len_name with (Int_val (i))))%CE.
+Definition wrap_max_len_fun := Fun [BNamed "i"] (wrap_max_len_code "i").
+Definition wrap_max_len_name := "wrap_max_len".
+
+Definition wrap_compress_code (bf1 bf2 : expr) : expr :=
+  let: "bts1" := Custom_contents(Field(Field(bf1, #1), #1)) in
+  let: "bts2" := Custom_contents(Field(Field(bf2, #1), #1)) in
+  let: "used1" := Int_val(Field(Field(bf1, #0), #0)) in
+  let: "cap2p" := malloc(#1) ;; "cap2p" <- Int_val(Field(Field(bf2, #1), #0)) in
+  let: "res" := call: &buffy_compress_name with ("bts1", "used1", "bts2", "cap2p") in
+  Store_field(&Field(Field(bf2, #0), #0), Val_int( *"cap2p")) ;;
+  free ("cap2p", #1) ;;
+  if: "res" = #0 then Val_int(#1) else Val_int(#0).
+Definition wrap_compress_fun := Fun [BNamed "bf1"; BNamed "bf2"] (wrap_compress_code "bf1" "bf2").
+Definition wrap_compress_name := "wrap_compress".
 
 End C_prog.
 
