theories/interop/wp_utils.v
@@ -30,31 +30,6 @@ Context `{!wrapperG Σ}.
 Implicit Types P : iProp Σ.
 Import mlanguage.
 
-(* TODO: auxiliary definition? *)
-Notation C_proto := (string -d> list Cval -d> (Cval -d> iPropO Σ) -d> iPropO Σ).
-Notation ML_proto := (string -d> list MLval -d> (MLval -d> iPropO Σ) -d> iPropO Σ).
-
-(* TODO: move *)
-Definition wrap_proto (Ψ : ML_proto) : C_proto := (λ f ws Φ,
-  ∃ θ vs lvs Φ',
-    "HGC" ∷ GC θ ∗
-    "%Hrepr" ∷ ⌜Forall2 (repr_lval θ) lvs ws⌝ ∗
-    "Hsim" ∷ lvs ~~∗ vs ∗
-    "Hproto" ∷ Ψ f vs Φ' ∗
-    "Cont" ∷ ▷ (∀ θ' vret lvret wret,
-      GC θ' -∗
-      Φ' vret -∗
-      lvret ~~ vret -∗
-      ⌜repr_lval θ' lvret wret⌝ -∗
-      Φ wret)
-)%I.
-
-Lemma wrap_proto_mono Ψ Ψ' : Ψ ⊑ Ψ' → wrap_proto Ψ ⊑ wrap_proto Ψ'.
-Proof using.
-  iIntros (Hre ? ? ?) "H". unfold wrap_proto. iNamed "H".
-  rewrite /named. iExists _, _, _, _. iFrame. iSplit; first done.
-  by iApply Hre.
-Qed.
 
 Section RootsRepr.
 
